Cslib/Computability/Automata/Deterministic/DA.lean
@@ -1,0 +1,39 @@
+/-
+Copyright (c) 2025 Fabrizio Montesi. All rights reserved.
+Released under Apache 2.0 license as described in the file LICENSE.
+Authors: Fabrizio Montesi
+-/
+
+import Cslib.Init
+
+/-! # Deterministic Automaton
+
+A Deterministic Automaton (DA) is an automaton defined by a transition function.
+-/
+
+namespace Cslib.Automata
+
+structure DA (State : Type _) (Symbol : Type _) where
+  /-- The initial state of the automaton. -/
+  start : State
+  /-- The transition function of the automaton. -/
+  tr : State → Symbol → State
+
+namespace DA
+
+variable {State : Type _} {Symbol : Type _}
+
+/-- Extended transition function.
+
+Implementation note: compared to [Hopcroft2006], the definition consumes the input list of symbols
+from the left (instead of the right), in order to match the way lists are constructed.
+-/
+@[scoped grind =]
+def mtr (da : DA State Symbol) (s : State) (xs : List Symbol) := xs.foldl da.tr s
+
+@[scoped grind =]
+theorem mtr_nil_eq {da : DA State Symbol} {s : State} : da.mtr s [] = s := rfl
+
+end DA
+
+end Cslib.Automata
