Cslib/Computability/Automata/Nondeterministic/EpsilonAcceptor.lean
@@ -1,0 +1,38 @@
+/-
+Copyright (c) 2025 Fabrizio Montesi. All rights reserved.
+Released under Apache 2.0 license as described in the file LICENSE.
+Authors: Fabrizio Montesi
+-/
+
+import Cslib.Computability.Automata.Nondeterministic.NA
+import Cslib.Computability.Automata.Acceptor
+
+namespace Cslib.Automata.NA
+
+variable {Symbol : Type _} {State : Type _}
+
+@[local grind =]
+private instance : HasTau (Option α) := ⟨.none⟩
+
+/-- The `ε`-closure of a set of states `S` is the set of states reachable by any state in `S`
+by performing only `ε`-transitions. We use `LTS.τClosure` since `ε` (`Option.none`) is an instance
+of `HasTau.τ`. -/
+abbrev εClosure (na : NA State (Option Symbol)) (S : Set State) := na.τClosure S
+
+/--
+Returns an acceptor that accepts a string if there is a saturated multistep accepting derivative
+with that trace from the start state.
+
+This is the standard string recognition performed by εNFAs in the literature.
+Formally, this is obtained by considering an `NA` with an `Option` symbol type.
+The special symbol `ε` is represented by the `Option.none` case.
+
+Internally, `ε` (`Option.none`) is treated as the `τ` label of the transition system of the `NA`,
+allowing for reusing the definitions and results on saturated transitions of `LTS` to deal with
+ε-closure.
+-/
+def εAcceptor (na : NA State (Option Symbol)) (acc : Set State) : Acceptor Symbol where
+  Accepts (xs : List Symbol) :=
+    ∃ s ∈ na.εClosure na.start, ∃ s' ∈ acc, na.saturate.MTr s (xs.map (some ·)) s'
+
+end Cslib.Automata.NA
